More simplifications.

withtop/Proofs/semantics/SemanticsSimpl.v
@@ -48,7 +48,6 @@ Inductive In : PExp -> PTyp -> Prop :=
   | InFun : forall e A B, In (PAnn CT (PLam e) (Fun A B)) (Fun A B)
   | InAnd : forall v1 v2 A B, In v1 A ->
                          In v2 B ->
-                         OrthoS A B ->
                          In (PMerge v1 v2) (And A B).
 
 Inductive bidityping : ST.context PTyp -> PExp -> Dir -> PTyp -> Prop :=
@@ -95,11 +94,15 @@ Inductive red : PExp -> PExp -> Prop :=
                  red e1 e3 ->
                  red (PApp e1 e2) (PApp e3 e2)
   | Red_App2 : forall e1 e2 v A B,
-                 ~ (In e1 A) ->
                  In v (Fun A B) ->
-                 red (PAnn CT e1 A) (PAnn CT e2 A) ->
+                 red e1 e2 ->
                  red (PApp v e1) (PApp v e2)
-  | Red_App3 : forall A B e v,
+  | Red_App3 : forall A B C v1 v2,
+                 In v1 (Fun A B) ->
+                 In v2 C ->
+                 A <> C ->
+                 red (PApp v1 v2) (PApp v1 (PAnn CT v2 C))
+  | Red_App4 : forall A B e v,
                  In v A -> 
                  red (PApp (PAnn CT (PLam e) (Fun A B)) v)
                      (PAnn CT (open_source e v) B)
@@ -112,15 +115,13 @@ Inductive red : PExp -> PExp -> Prop :=
                    red (PMerge v e1) (PMerge v e2)
   | Red_Ann1 : forall e1 e2 A,
                  ~ (In (PAnn CT e1 A) A) ->
-                 ~ In e1 A ->
                  red e1 e2 ->
                  red (PAnn CT e1 A) (PAnn CT e2 A)
-  | Red_Ann2 : forall A v,
-                 In v A ->
-                 red (PAnn CT v A) v
-  | Red_Ann3Abs :
+  | Red_Ann2 : forall v,
+                 In v PInt ->
+                 red (PAnn CT v PInt) v
+  | Red_Ann3 :
       forall e A B C D,
-        Fun A B <> Fun C D ->
         red (PAnn CT (PAnn CT (PLam e) (Fun A B)) (Fun C D))
             (PAnn CT (PLam (PAnn CT (PApp (PAnn CT (PLam e) (Fun A B))
                                           (PAnn CT (PBVar 0) A)) D))
@@ -139,7 +140,6 @@ Inductive red : PExp -> PExp -> Prop :=
                      (PAnn CT v2 A)
   | Red_Ann6 : forall v A B C D,
                  In v (And C D) ->
-                 (And C D) <> (And A B) ->
                  red (PAnn CT v (And A B))
                      (PMerge (PAnn CT v A) (PAnn CT v B)).
 
@@ -241,44 +241,36 @@ Proof. intros v A B H1; dependent induction H1; auto. Qed.
 Hint Resolve In_Ann_inv.
 Hint Unfold erase.
 
-Theorem In_bityping_sub :
-  forall A v, In v A -> forall B Gamma, bidityping Gamma v Inf B -> Sub A B.
+Theorem In_bityping_eq :
+  forall A v, In v A -> forall B Gamma, bidityping Gamma v Inf B -> A = B.
 Proof.
   intros A v HIn.
   induction HIn; eauto 3.
   - intros; inversion H; subst; eauto.
   - intros; inversion H; subst; eauto.
-  - intros; dependent induction H0.
+  - intros. dependent induction H.
     clear IHbidityping1 IHbidityping2.
-    apply IHHIn1 in H0_.
-    apply IHHIn2 in H0_0.
-    auto.
+    apply IHHIn1 in H.
+    apply IHHIn2 in H0.
+    now subst.
+Qed.
+
+Hint Resolve In_bityping_eq.
+
+Theorem In_bityping_sub :
+  forall A v, In v A -> forall B Gamma m, bidityping Gamma v m B -> Sub A B.
+Proof.
+  intros A v HIn.
+  induction HIn. 
+  - intros; inversion H; subst; auto.
+    inversion H0; subst; eauto.
+  - intros; inversion H; subst; auto.
+    inversion H0; subst; eauto.
+  - intros; dependent induction H; [ clear IHbidityping1 IHbidityping2 | eauto 5 ].
+    apply sand1; [ apply sand2 | apply sand3 ]; eauto.
 Qed.
 
 Hint Resolve In_bityping_sub.
-
-Theorem In_bityping :
-  forall Gamma A B e, In e A -> bidityping Gamma e Inf B -> bidityping Gamma e Inf A.
-Proof.
-  intros Gamma A B e HIn Htyping.
-  assert (HSub : Sub A B) by eauto.
-  generalize dependent A.
-  induction Htyping; intros; try now inversion HIn.
-  - apply invAndS1 in HSub. destruct HSub.
-    inversion HIn; subst.
-    assert (Ha1 : Sub A1 A) by eauto.
-    assert (Ha2 : Sub B0 B) by eauto.
-    assert (Ha3 : bidityping Gamma t1 Inf A1) by auto.
-    assert (Ha4 : bidityping Gamma t2 Inf B0) by auto.
-    auto. (* since Value implies disjointness *)
-  - inversion HIn; subst; eauto.
-  - assert (Ha1 : Sub A0 A) by eauto.
-    assert (Ha2 : bidityping Gamma t0 Inf A0) by auto.
-    assert (Ha3 : Sub A0 A0) by apply reflex.
-    destruct Ha3; eauto.
-Qed.  
-
-Hint Resolve In_bityping.
 
 Theorem bityping_inf_chk :
   forall Gamma e A,
@@ -359,13 +351,15 @@ Proof.
   intros Gamma e1 A m Htyping e2 Hred;
   generalize dependent A; generalize dependent Gamma; generalize dependent m.
   induction Hred; intros; try now (dependent induction Htyping; subst; eauto).
-  - (* R_App2 *)
-    dependent induction Htyping; subst; eauto; clear IHHtyping1 IHHtyping2.
-    inversion H0; subst; inversion Htyping1; subst.
-    apply ATyApp' with (A := A0); auto.
-    assert (Ha : bidityping Gamma (PAnn CT e1 A0) Inf A0) by eauto.
-    apply IHHred in Ha; inversion Ha; now subst.
   - (* R_App3 *)
+    dependent induction Htyping; subst; eauto; clear IHHtyping1 IHHtyping2.
+    inversion H; subst; inversion Htyping1; subst.
+    apply ATyApp' with (A := A0); auto.
+    inversion Htyping2; subst.
+    inversion H0.
+    assert (Ha : C = A) by eauto; subst.
+    eapply ATySub' with (A := A); eauto.
+  - (* R_App4 *)
     dependent induction Htyping; subst; eauto.
     clear IHHtyping1 IHHtyping2.
     inversion Htyping1; subst.
@@ -375,24 +369,25 @@ Proof.
     inversion H0.
     dependent induction Htyping2; subst; eauto.
     inversion H2.
+    assert (B = A) by eauto; now subst.
   - (* R_Ann2 *)
     dependent induction Htyping; eauto; subst; clear IHHtyping.
     dependent induction Htyping; eauto.
-    inversion H2. 
+    inversion H1; subst; eauto.
   - (* R_AnnAbs *)
     dependent induction Htyping; subst; eauto; clear IHHtyping.
     inversion Htyping; subst.
-    inversion H0; subst.
-    inversion H2; subst.
+    inversion H; subst.
+    inversion H1; subst.
     apply ATyAnnCT'.     
     apply_fresh ATyLam' as x; auto.
     unfold open_source; simpl.
     assert (Ha : Sub D D) by apply reflex; destruct Ha.
     assert (Ha : WFTyp A) by
-        (now assert (Ha := bityping_wf _ _ _ _ H0); inversion Ha).
+        (now assert (Ha := bityping_wf _ _ _ _ H); inversion Ha).
     eapply ATySub' with (A := D); eauto 2.
     apply ATyAnnCT'.
-    inversion H1; subst; clear H1.
+    inversion H0; subst; clear H0.
     eapply ATySub' with (A := B); eauto 2.
     eapply ATyApp' with (A := A).
     + apply ATyAnnCT'.
@@ -415,16 +410,18 @@ Proof.
     dependent induction Htyping; subst; eauto; clear IHHtyping.
     destruct H.
     inversion Htyping; subst.
-    inversion H2; inversion H1; subst; eauto.
+    inversion H2; inversion H1; subst.
+    assert (B = A1) by eauto; subst; eauto.    
   - (* R_Ann5 *)
     dependent induction Htyping; subst; eauto; clear IHHtyping.
     destruct H.
     inversion Htyping; subst.
-    inversion H2; inversion H1; subst; eauto.
+    inversion H2; inversion H1; subst.
+    assert (C = B0) by eauto; subst; eauto.
   - (* R_Ann6 *)
     dependent induction Htyping; subst; eauto; clear IHHtyping.
     inversion Htyping; subst.
-    inversion H2; subst; try now inversion H5.
+    inversion H1; subst; try now inversion H4.
     assert (Ha : WFTyp (And A B)) by eauto; inversion Ha; subst.
     assert (Ha2 : Sub A0 A) by eauto.
     assert (Ha3 : Sub A0 B) by eauto.
@@ -457,19 +454,18 @@ Lemma In_unique : forall v A B, In v A -> In v B -> A = B.
 Proof.
   intros v A B HIn1 HIn2. generalize dependent B.
   induction HIn1; intros; inversion HIn2; subst; auto.
-  apply IHHIn1_1 in H2.
-  apply IHHIn1_2 in H3.
-  now subst.
+  apply IHHIn1_1 in H1; apply IHHIn1_2 in H3; now subst.
 Qed.
 
 Hint Rewrite In_unique.
-    
+
+(*
 Lemma value_ann_red_id :
   forall v A e, In v A -> red (PAnn CT v A) e -> v = e.
 Proof.
   intros v A e Hin Hred.
   dependent induction Hred; eauto.
-  - inversion Hin; subst; exfalso; now apply H.
+  - inversion Hin; subst; exfalso. now apply H.
   - inversion Hin; subst; inversion H0.
   - inversion Hin; subst; inversion H0.
   - inversion Hin; subst.
@@ -478,60 +474,78 @@ Proof.
 Qed.
 
 Hint Rewrite value_ann_red_id.
+*)
 
 Theorem red_unique :
-  forall e1 e2, red e1 e2 -> forall e3, red e1 e3 -> e2 = e3.
+  forall e1 e2, red e1 e2 -> forall e3, red e1 e3 -> forall Gamma A m, bidityping Gamma e1 m A -> e2 = e3.
 Proof.
   intros e1 e2 Hred.
   induction Hred; intros.
   - inversion H; subst; auto.
   - inversion H; subst; auto.
-    + apply IHHred in H3; now subst.
+    + dependent induction H0; subst; eauto; clear IHbidityping1 IHbidityping2.
+      eapply IHHred in H4; subst; eauto.
     + inversion Hred; subst; auto.
   - inversion H0; subst.
     inversion H1; subst; auto.
-    + assert (Ha : Fun A B = Fun A0 B0) by eauto; inversion Ha; subst.
-      apply IHHred in H7; inversion H7; now subst.
-    + contradiction.
+    + dependent induction H1; eauto. clear IHbidityping1 IHbidityping2.
+      eapply IHHred in H6; subst; eauto.
+    + dependent induction H1; eauto.
+    + dependent induction H1; eauto.
+  - inversion H2; subst; auto.
+    + assert (Ha : C = C0) by (eapply In_unique; eauto); subst; auto.
+    + assert (Ha : Fun A1 B0 = Fun A B) by (eapply In_unique; eauto).
+      inversion Ha; subst.
+      assert (Ha1 : A = C) by (eapply In_unique; eauto); subst.
+      exfalso; apply H1; auto.
   - inversion H0; subst; auto.
-    + inversion H4; subst; auto. 
-    + inversion H4; subst; contradiction.
+    + inversion H5; subst; auto. 
+    + inversion H4; subst.
+      assert (Ha1 : A1 = C) by (eapply In_unique; eauto); subst.
+      exfalso; apply H7; auto.
   - inversion H; subst; auto.
-    + apply IHHred in H3; now subst.
+    + dependent induction H0; eauto; clear IHbidityping1 IHbidityping2.
+      eapply IHHred in H4; subst; eauto.
   - inversion H; subst.
+    dependent induction H1; eauto; clear IHbidityping1 IHbidityping2.
     inversion H; inversion H0; subst; auto.
-    apply IHHred in H15; now subst.
-  - inversion H1; subst; auto; try now (inversion Hred; subst; auto).
-    + apply IHHred in H7; now subst.
-  - inversion H0; subst; auto.
-    assert ((Fun A0 B) = (Fun C D)) by eauto; contradiction.
-    inversion H; subst; inversion H4.
-    inversion H; subst; inversion H4.
-    assert (Ha : And C D = And A0 B) by (eapply In_unique; eauto); inversion Ha; subst.
-    exfalso; now apply H5.
-  - inversion H0; subst; auto.
-    inversion H6; subst; auto.
-    assert ((Fun A B) = (Fun C D)) by eauto; contradiction.
+    eapply IHHred in H14; subst; eauto.
+  - dependent induction H0; eauto.
+    clear IHred.
+    dependent induction H2; eauto 3; clear IHbidityping.
+    eapply IHHred in H0; subst; eauto.
+    inversion H1; subst; inversion Hred; subst; auto.
+  - inversion H0; subst; auto; inversion H.
+  - dependent induction H; eauto.
+    assert (Ha : In (PAnn CT (PLam e) (Fun A B)) (Fun A B)) by auto.
+    apply (value_not_red _ _ _ Ha) in H0; exfalso; auto.
   - inversion H1; subst.
     dependent induction H2; subst; auto.
     inversion H2; subst; inversion H0.
+    dependent induction H5; subst; eauto 3; clear IHbidityping.
     assert (Ha : And B C = And B0 C0) by (eapply In_unique; eauto); inversion Ha; subst.
+    inversion H5; subst.
+    assert (Ha1 : A0 = And B0 C0) by (symmetry; eauto); subst.
+    inversion H6; subst.
     assert (Ha1 : ~ (Sub C0 A /\ Sub B0 A)) by eauto.
     exfalso; apply Ha1; split; assumption.
     inversion H0.
   - inversion H1; subst.
     dependent induction H2; subst; auto.
     inversion H2; subst; inversion H0.
+    dependent induction H5; subst; eauto 3; clear IHbidityping.
     assert (Ha : And B C = And B0 C0) by (eapply In_unique; eauto); inversion Ha; subst.
+    inversion H5; subst.
+    assert (Ha1 : A0 = And B0 C0) by (symmetry; eauto); subst.
+    inversion H6; subst.
     assert (Ha1 : ~ (Sub C0 A /\ Sub B0 A)) by eauto.
     exfalso; apply Ha1; split; assumption.
     inversion H0.
-  - inversion H; subst.
-    inversion H1; subst; auto.
-    assert (Ha : And C D = And A B) by (eapply In_unique; eauto); inversion Ha; subst. 
-    exfalso; now apply H0.
-    inversion H10.
-    inversion H10.    
+  - inversion H0; subst.
+    inversion H0; subst; auto.
+    inversion H5.
+    inversion H5.
+    reflexivity.
 Qed.
       
 (** Theorem 3. All typeable terms can reduce **)
@@ -551,10 +565,13 @@ Proof.
     destruct Ha2.
     destruct H2.
     inversion H1; subst.
-    assert (Ha : red ( 
     admit. (* *)
-    eauto.
     admit.
+  - admit.
+  - admit.
+  - admit.
+  - admit.
+  - admit.
 Admitted.
 
 End Semantics.
